\documentclass{jsarticle}

\usepackage{amsmath, amssymb, amsthm}
\usepackage{enumerate}

\parindent = 0pt

\begin{document}
    
    $P(x, y, z) = y^2z - x(x-z)(x-\lambda z)$ とする。ただし $\lambda \in \mathbb{C}$.
    
    \begin{align*}
        \mathcal{H}_P & = \begin{pmatrix}
            -6x + 2(\lambda + 1)z & 0 & 2(\lambda+1)x-2\lambda z\\
            0 & 2z & 2y\\
            2(\lambda+1)x-2\lambda z & 2y & 2\lambda x
        \end{pmatrix}\\
        & = 8(\lambda xz((\lambda+1)z-3x) - ((\lambda+1)x - \lambda z)^2z - ((\lambda+1)z-3x)y^2).
    \end{align*}
    
    この式の $xy^2$ の項に着目して
    $$(\mathcal{H}_P)_x(0,1,0) = 8 \times 3 = 24$$.
    

\end{document}